low/Relation.v
@@ -1,0 +1,4 @@
+(** Relation.
+* Links the low-level formalisation to the C source code of R. **)
+
+(* TODO *)
