low/Reval.v
@@ -1,6 +1,6 @@
 (** Reval.
 * Describes how R evaluates expressions.
-* The content of this file is the Coq equivalent of the file src/main/eval.c. **)
+* The content of this file is the Coq equivalent of the file src/main/eval.c from R source code. **)
 
 Set Implicit Arguments.
 Require Export Monads.
@@ -9,23 +9,104 @@ Require Export Monads.
 
 (** A structure to deal with infinite execution (which is not allowed in Coq). Inspired from JSCert. **)
 Record runs_type : Type := runs_type_intro {
+    runs_fold_left_listSxp : forall A, state -> SExpRec_pointer -> A ->
+      (state -> A -> SExpRec_pointer -> SExpRec_pointer -> result A) -> result A ;
     runs_eval : state -> SExpRec_pointer -> SExpRec_pointer -> result SExpRec_pointer
   }.
 
 
 (** * Interpreter functions **)
 
+(** The C language performs a lot of pointer deferentiation. As a
+* convention, we write [p_] for the object referenced by the pointer [p]
+* in this section, and [p_f] for the field [f] or it, typically [p_sym]
+* for its [symSxp_struct] part and so on. **)
+
+(** ** Frequent Pattern **)
+
+(** The functions presented here are not from R source code, but
+ * represent frequent programming pattern in its source code. **)
+
+(** Looping through a list is a frequent pattern in R source code.
+ * [fold_left_listSxp] corresponds to the C code
+ * [for (i = l, v = a; i != R_NilValue; i = CDR (i)) v = iterate (CAR (i), TAG (i), v); v]. **)
+Definition fold_left_listSxp A runs (S : state) (l : SExpRec_pointer) (a : A)
+    (iterate : state -> A -> SExpRec_pointer -> SExpRec_pointer -> result A) : result A :=
+  ifb l = None then
+    result_success S a
+  else
+    if_defined S (read_SExp S l) (fun l_ =>
+      if_defined S (get_listSxp l_) (fun l_list =>
+        if_success (iterate S a (list_carval l_list) (list_tagval l_list)) (fun S a =>
+          runs_fold_left_listSxp runs S (list_cdrval l_list) a iterate))).
+
+(** ** memory.c **)
+
+(** The function names of this section corresponds to the function names
+* in the file src/main/memory.c. **)
+
+Definition CONS_NR (S : state) (car cdr : SExpRec_pointer) : state * SExpRec_pointer :=
+  let e_ := make_SExpRec (build_SExpRecHeader ListSxp None) (make_ListSxp_struct car cdr None) in
+  alloc_SExp S e_.
+
+(* Question: there is a point at which there is just too much details.
+ * There is no point in translating the entire R source code,
+ * even if we are skipping R functions.
+ * It is fine to understand what a given function does without translating
+ * exactly its source code. *)
+
+
+(** ** match.c **)
+
+(** The function names of this section corresponds to the function names
+* in the file src/main/match.c. **)
+
+(* Understanding C code can be trikky. Here are some hints.
+* psmatch (s1, s2, TRUE) is exactly s1 = s2
+* psmatch (s1, s2, FALSE) is exactly String.prefix s1 s2 *)
+
+(** The function [matchArgs] matches the arguments supplied to a given
+* call with the formal, expected arguments.
+* This is more complex as it may seem as arguments in R can be named
+* (and thus provided in any order), or can be ‘...’.
+* The algorithm presented in this function is thus crucial to understand
+* the semantics of function calls in R.
+* It is furthermore rather complicated. **)
+Definition matchArgs runs (S : state)
+    (formals supplied call : SExpRec_pointer) : SExpRec_pointer :=
+  (* TODO: fold_left_listSxp *)
+  .
+
+(** ** eval.c **)
+
+(** The function names of this section corresponds to the function names
+* in the file src/main/eval.c. **)
+
+(** The function [forcePromise] evaluates a promise if needed. **)
 Definition forcePromise runs (S : state) (e : SExpRec_pointer) : result SExpRec_pointer :=
-  if_defined S (read_SExp S e) (fun exp =>
-    if_defined S (get_promSxp exp) (fun p =>
-      If prom_value p = R_UnboundValue then
-        runs_eval runs S (prom_expr p) (prom_env p)
+  if_defined S (read_SExp S e) (fun e_ =>
+    if_defined S (get_promSxp e_) (fun e_prom =>
+      If prom_value e_prom = R_UnboundValue then
+        runs_eval runs S (prom_expr e_prom) (prom_env e_prom)
       else result_success S e)).
 
-(** The eval function of https://github.com/wch/r-source/blob/trunk/src/main/eval.c#L538 **)
+Definition applyClosure runs (S : state)
+    (call op arglist rho suppliedvars : SExpRec_pointer) : result SExpRec_pointer :=
+  if_defined S (read_SExp S rho) (fun rho_ =>
+    ifb type rho_ <> EnvSxp then
+      result_impossible S "[applyClosure] ‘rho’ must be an environment."
+    else
+      if_defined S (read_SExp S op) (fun op_ =>
+        if_defined S (get_cloSxp op_) (fun op_clo =>
+          let formals := clo_formals op_clo in
+          let savedrho := clo_env op_clo in
+          (* TODO : formals *)
+          result_not_implemented "[applyClosure]"))).
+
+(** The function [eval] evaluates its argument to an unreducible value. **)
 Definition eval runs (S : state) (e rho : SExpRec_pointer) : result SExpRec_pointer :=
-  if_defined S (read_SExp S e) (fun exp =>
-    match type exp with
+  if_defined S (read_SExp S e) (fun e_ =>
+    match type e_ with
     | NilSxp
     | ListSxp
     | LglSxp
@@ -43,13 +124,14 @@ Definition eval runs (S : state) (e rho : SExpRec_pointer) : result SExpRec_poin
     | ExtptrSxp
     | WeakrefSxp
     | ExprSxp =>
-      if_defined S (write_SExp S e (set_named exp)) (fun S =>
+      if_defined S (write_SExp S e (set_named e_)) (fun S =>
         result_success S e)
     | _ =>
-      if_defined S (read_SExp S rho) (fun env =>
-        match type exp with
-        | EnvSxp =>
-          match type exp with
+      if_defined S (read_SExp S rho) (fun rho_ =>
+        ifb type rho_ <> EnvSxp then
+          result_impossible S "[eval] ‘rho’ must be an environment."
+        else
+          match type e_ with
           | BcodeSxp =>
             (** See https://github.com/wch/r-source/blob/trunk/src/main/eval.c#L3543
              * for a definition of this bytecode, and
@@ -66,22 +148,22 @@ Definition eval runs (S : state) (e rho : SExpRec_pointer) : result SExpRec_poin
              * about these two functions. **)
             result_not_implemented "[eval] Symbols (TODO)"
           | PromSxp =>
-            if_defined S (get_promSxp exp) (fun p =>
-              ifb prom_value p = R_UnboundValue then
+            if_defined S (get_promSxp e_) (fun e_prom =>
+              ifb prom_value e_prom = R_UnboundValue then
                 if_success (forcePromise runs S e) (fun S e =>
                   result_success S e)
               else result_success S e)
           | LangSxp =>
-            if_defined S (get_listSxp exp) (fun l =>
-              let pcar := list_carval l in
-              if_defined S (read_SExp S pcar) (fun car =>
+            if_defined S (get_listSxp e_) (fun e_list =>
+              let car := list_carval e_list in
+              if_defined S (read_SExp S car) (fun car_ =>
                 if_success
-                  (ifb type car = SymSxp then
+                  (ifb type car_ = SymSxp then
                      (* TODO: findFun3 — in essence, this is just a variable look-up. *)
                      result_not_implemented "[eval] findFun3 (TODO)"
-                   else runs_eval runs S pcar rho) (fun S op =>
-                  if_defined S (read_SExp S op) (fun opp =>
-                    match type opp with
+                   else runs_eval runs S car rho) (fun S op =>
+                  if_defined S (read_SExp S op) (fun op_ =>
+                    match type op_ with
                     | SpecialSxp =>
                       (* TODO: This is basically a direct call to PRIMFUN. *)
                       result_not_implemented "[eval] PRIMFUN (TODO)"
@@ -95,15 +177,10 @@ Definition eval runs (S : state) (e rho : SExpRec_pointer) : result SExpRec_poin
                       result_not_implemented "[eval] applyClosure (TODO)"
                     | _ => result_error S "[eval] Attempt to apply non-function."
                     end))))
-          | DotSxp => result_error S "[eval] ‘...’ used in an incorrect context"
+          | DotSxp => result_impossible S "[eval] ‘...’ used in an incorrect context"
           | _ => result_error S "[eval] Type unimplemented in the R source code."
-          end
-        | _ => result_error S "[eval] ‘rho’ must be an environment."
-        end)
+          end)
     end).
-
-(** The property we want to eventually prove is that if [eval] returns
-  a result, then the C function eval does similarly. **)
 
 
 (** * Closing the loop **)
@@ -111,12 +188,23 @@ Definition eval runs (S : state) (e rho : SExpRec_pointer) : result SExpRec_poin
 Fixpoint runs max_step : runs_type :=
   match max_step with
   | O => {|
+      runs_fold_left_listSxp := fun _ S _ _ _ => result_bottom S ;
       runs_eval := fun S _ _ => result_bottom S
     |}
   | S max_step =>
     let wrap {A : Type} (f : runs_type -> A) : A :=
       f (runs max_step) in {|
+      runs_fold_left_listSxp := wrap fold_left_listSxp ;
       runs_eval := wrap eval
     |}
   end.
+
+
+(** * Proofs **)
+
+(** It would be nice to prove that the read-eval-print-loop can not
+* return a [result_impossible]. **)
+
+(** The property we want to eventually prove is that if [eval] returns
+* a result, then the C function eval does similarly. **)
 
