high/Relation.v
@@ -1,0 +1,4 @@
+(** Relation.
+* Links the high-level formalisation to the structured-level one. **)
+
+(* TODO *)
